src/HighValues.v
@@ -1,0 +1,507 @@
+Require Import compcert.lib.Coqlib.
+Require Import compcert.lib.Maps.
+Require Import compcert.lib.Integers.
+
+Require Import compcert.common.AST.
+Require Import compcert.common.Values.
+Require Import compcert.common.Globalenvs.
+Require Import compcert.common.Memory.
+Require Import compcert.common.Events.
+Require Import compcert.common.Switch.
+Require Import compcert.common.Smallstep.
+
+Require Import List.
+Import ListNotations.
+Require Import Arith.
+Require Import Ring.
+
+Require Import StructTact.StructTactics.
+Require Import StructTact.Util.
+
+
+(* Computation will be over higher level values, i.e. Constr and Close *)
+(* We will need a way to relate those to lower level values *)
+(* That relation will have type hval -> rval -> mem -> Prop *)
+(* since high level values will have to live in memory *)
+
+Definition function_name := ident.
+
+Inductive value :=
+| Constr (tag : int) (args : list value) (* A constructor applied to some values *)
+(* At this level we have a Z tag  *)
+(* corresponds with lower level switch semantics nicely *)
+| Close (f : function_name) (free : list value). (* a closure value *)
+(* free is the list of values closed over, referred to inside as upvars *)
+
+(* Thanks Stuart *)
+Definition value_rect_mut (P : value -> Type) (Pl : list value -> Type)
+           (HConstr : forall tag args, Pl args -> P (Constr tag args))
+           (HClose : forall fname args, Pl args -> P (Close fname args))
+    (Hnil :     Pl [])
+    (Hcons :    forall e es, P e -> Pl es -> Pl (e :: es))
+    (v : value) : P v :=
+    let fix go v :=
+        let fix go_list vs :=
+            match vs as vs_ return Pl vs_ with
+            | [] => Hnil
+            | v :: vs => Hcons v vs (go v) (go_list vs)
+            end in
+        match v as v_ return P v_ with
+        | Constr tag args => HConstr tag args (go_list args)
+        | Close f args => HClose f args (go_list args)
+        end in go v.
+
+(* Useful wrapper for `expr_rect_mut with (Pl := Forall P)` *)
+Definition value_ind' (P : value -> Prop) 
+           (HConstr : forall tag args, Forall P args -> P (Constr tag args))
+           (HClose : forall fname args, Forall P args -> P (Close fname args))
+    (v : value) : P v :=
+    ltac:(refine (@value_rect_mut P (Forall P)
+        HConstr HClose _ _ v); eauto).
+
+
+(* given an address, addresses of the nested values *)
+Fixpoint arg_addrs (b : block) (ofs : int) (l : list value) : list (value * val) :=
+  match l with
+  | nil => nil
+  | v :: vs =>
+    let ofs' := Int.add ofs (Int.repr 4) in
+    (v, Vptr b ofs) :: arg_addrs b ofs' vs
+  end.
+
+Fixpoint load_all (l : list (value * val)) (m : mem) : option (list (value * val)) :=
+  match l with
+  | nil => Some nil
+  | (hval,vaddr) :: rest =>
+    match Mem.loadv Mint32 m vaddr with
+    | None => None
+    | Some v' =>
+      match load_all rest m with
+      | None => None
+      | Some res => Some ((hval,v') :: res)
+      end
+    end
+  end.
+                     
+
+(* mapping of high level values to low level values *)
+(* everything is one pointer *)
+Inductive value_inject {A B} (ge : Genv.t A B) (m : mem) : value -> val -> Prop :=
+| inj_constr :
+    (* a constructor is a pointer to the correct tag *)
+    (* and every value following that in memory is a value for that constructor *)
+    (* *(b,ofs) = tag *)
+    (* *(b,ofs+4) = pointer to first field *)
+    forall b ofs n values l',
+      Mem.loadv Mint32 m (Vptr b ofs) = Some (Vint n) -> (* correct tag *)
+      load_all (arg_addrs b (Int.add ofs (Int.repr 4)) values) m = Some l' -> (* one more deref for args *)
+      (forall a b, In (a,b) l' -> value_inject ge m a b) -> (* all args inject *)
+      value_inject ge m (Constr n values) (Vptr b ofs)
+| inj_closure :
+    forall b ofs bcode f fname values l',
+      Mem.loadv Mint32 m (Vptr b ofs) = Some (Vptr bcode Int.zero) ->
+      Genv.find_funct_ptr ge bcode = Some f -> (* legit pointer to some code *)
+      Genv.find_symbol ge fname = Some bcode -> (* name we have points to same code *)
+      load_all (arg_addrs b (Int.add ofs (Int.repr 4)) values) m = Some l' -> (* one more deref for args *)
+      (forall a b, In (a,b) l' -> value_inject ge m a b) -> (* all args inject *)
+      value_inject ge m (Close fname values) (Vptr b ofs).
+
+
+Definition env_inject {A B} (hlenv : PTree.t value) (llenv : PTree.t val) (ge : Genv.t A B)(m : mem) : Prop :=
+  forall id v,
+    PTree.get id hlenv = Some v ->
+    exists v',
+      PTree.get id llenv = Some v' /\ value_inject ge m v v'.
+  
+
+Lemma load_all_val :
+  forall l b ofs m l' n v,
+    nth_error l n = Some v ->
+    load_all (arg_addrs b ofs l) m = Some l' ->
+    exists v',
+      Mem.loadv Mint32 m (Vptr b (Int.add ofs (Int.repr (4 * Z.of_nat n)))) = Some v' /\ In (v,v') l'.
+Proof.
+  induction l; intros;
+    destruct n; simpl in H; inv H; subst.
+  * simpl in H0.
+    repeat break_match_hyp; try congruence.
+    simpl. replace (Int.add ofs (Int.repr 0)) with ofs by ring.
+    eexists; split; eauto. invc H0. simpl.
+    left. auto.
+  * simpl in H0. repeat break_match_hyp; try congruence.
+    inv H0.
+    eapply IHl in H; eauto.
+    repeat break_exists; repeat break_and.
+    replace (Int.add (Int.add ofs (Int.repr 4)) (Int.repr (4 * Z.of_nat n)))
+    with  (Int.add ofs (Int.repr (4 * Z.of_nat (S n)))) in H.
+    
+    eexists. split. eauto.
+    simpl. right. auto.
+
+    (* rest is annoying math over Z/nat/int *)
+    replace (4 * Z.of_nat (S n)) with (4 + 4 * Z.of_nat n)%Z.
+    rewrite Int.add_assoc.
+    f_equal.
+    rewrite Int.add_unsigned.
+    rewrite (Int.unsigned_repr 4).
+    rewrite Int.unsigned_repr_eq.
+    eapply Int.eqm_samerepr.
+    unfold Int.eqm.
+    assert (Int.modulus > 0).
+    unfold Int.modulus, two_power_nat, Int.wordsize, Wordsize_32.wordsize.
+    simpl. omega.
+    remember (Int.eqmod_mod Int.modulus H3) as ie.
+    eapply Int.eqmod_add. econstructor; eauto. instantiate (1 := 0).
+    omega.
+    eapply Int.eqmod_mod.
+    omega. unfold Int.max_unsigned.
+    simpl. omega.
+    rewrite Nat2Z.inj_succ.
+    omega.
+Qed.
+
+
+
+(* (* number of bytes to store a value *) *)
+Definition size_bytes (v : value) : Z :=
+  match v with
+  | Close _ l => (4 * Z.of_nat (length l)) + 4
+  | Constr _ l => (4 * Z.of_nat (length l)) + 4
+  end.
+
+
+(* Definition first_byte (v : value) : option val := *)
+(*   match v with *)
+(*   | Close fname _ => *)
+(*     match Genv.find_symbol tge fname with *)
+(*     | Some b => Some (Vptr b Int.zero) *)
+(*     | None => None *)
+(*     end *)
+(*   | Constr tag _ => Some (Vint tag) *)
+(*   end. *)
+
+(* Definition rest (v : value) : list value := *)
+(*   match v with *)
+(*   | Close _ l => l *)
+(*   | Constr _ l => l *)
+(*   end. *)
+
+Section sv.
+
+  Variable A B : Type.
+
+  
+Fixpoint store_value (ge : Genv.t A B) (v : value) (m : mem) {struct v} : option (val * mem) :=
+  let fix store_values ge b ofs l m :=
+      match l with
+      | nil => Some m
+      | v :: vs =>
+        match store_values ge b (ofs + 4)%Z vs m with
+        | Some m' =>
+          match store_value ge v m' with
+          | Some (vp,m'') => Mem.storev Mint32 m'' (Vptr b (Int.repr ofs)) vp
+          | None => None
+          end
+        | None => None
+        end
+      end in
+  let sz := size_bytes v in (* find total size for value *)
+  let (m',b) := Mem.alloc m 0 sz in (* allocate that much space *)
+  match v with
+  | Close fname l =>
+    match Genv.find_symbol ge fname with
+    | Some bcode =>
+      match Genv.find_funct_ptr ge bcode with
+      | Some _ =>
+        match Mem.storev Mint32 m' (Vptr b Int.zero) (Vptr bcode Int.zero) with
+        | Some m'' =>
+          match store_values ge b 4 l m'' with
+          | Some m''' => Some (Vptr b Int.zero, m''')
+          | None => None
+          end
+        | None => None
+        end
+      | None => None
+      end
+    | None => None
+    end
+  | Constr tag l =>
+    match Mem.storev Mint32 m' (Vptr b Int.zero) (Vint tag) with
+    | Some m'' =>
+      match store_values ge b 4 l m'' with
+      | Some m''' => Some (Vptr b Int.zero, m''')
+      | None => None
+      end
+    | None => None
+    end
+  end.
+
+(* implicit argument magic *)
+Global Arguments store_value : default implicits.
+
+Fixpoint store_values (ge : Genv.t A B) (b : block) (ofs : Z) (l : list value) (m : mem) :=
+      match l with
+      | nil => Some m
+      | v :: vs =>
+        match store_values ge b (ofs + 4)%Z vs m with
+        | Some m' =>
+          match store_value ge v m' with
+          | Some (vp,m'') => Mem.storev Mint32 m'' (Vptr b (Int.repr ofs)) vp
+          | None => None
+          end
+        | None => None
+        end
+      end.
+
+(* implicit argument magic *)
+Global Arguments store_values : default implicits.
+
+End sv.
+
+Definition all_addrs (b : block) (z : Z) : Prop := True.
+
+Lemma store_value_unchanged :
+  forall {A B} v m v' m' (ge : Genv.t A B),
+    store_value ge v m = Some (v',m') ->
+    Mem.unchanged_on all_addrs m m'.
+Proof.
+  induction v using value_ind'; intros; econstructor; intros;
+    simpl in *;
+    repeat (break_match_hyp; try congruence);
+  assert (~ Mem.valid_block m b0);
+    try (eapply Mem.fresh_block_alloc; eauto);
+    destruct (peq b b0); try congruence;
+  match goal with
+  | [ H : Mem.perm _ _ _ _ _ |- _ ] => eapply Mem.perm_valid_block in H; congruence
+  | [ |- _ ] => idtac
+  end.
+
+  (* at least now we know that b <> b0 *)
+  (* now we have to show that nothing happened elsewhere *)
+  
+Admitted.
+
+Lemma loadv_unchanged_on :
+  forall m m',
+    Mem.unchanged_on all_addrs m m' ->
+    forall c v v',
+      Mem.loadv c m v = Some v' ->
+      Mem.loadv c m' v = Some v'.
+Proof.
+  intros.
+  unfold Mem.loadv in H0.
+  break_match_hyp; try congruence.
+  subst v.
+  simpl.
+  eapply Mem.load_unchanged_on; eauto.
+  intros. unfold all_addrs. auto.
+Qed.
+
+Lemma load_all_unchanged_on :
+  forall m m',
+    Mem.unchanged_on all_addrs m m' ->
+    forall l l',
+      load_all l m = Some l' ->
+      load_all l m' = Some l'.
+Proof.
+  induction l; intros.
+  simpl in H0. inv H0. simpl. reflexivity.
+  simpl in H0.
+  repeat break_match_hyp; try congruence. subst a.
+  invc H0. simpl.
+  erewrite loadv_unchanged_on; eauto.
+  erewrite IHl; eauto.
+Qed.
+
+Lemma value_inject_load_all :
+  forall {A B} args b ofs m l' (ge : Genv.t A B),
+    load_all (arg_addrs b ofs args) m = Some l' ->
+    forall m m',
+      Forall (fun v => forall v', value_inject ge m v v' -> value_inject ge m' v v') args ->
+      forall a b,
+        In (a,b) l' ->
+        value_inject ge m a b ->
+        value_inject ge m' a b.
+Proof.
+  induction args; intros.
+  simpl in H. inv H. simpl in H1.
+  inv H1.
+  simpl in H.
+  repeat break_match_hyp; try congruence. invc H.
+  simpl in H1.
+  destruct H1.
+  * invc H. inv H0. eapply H3. eauto.
+  * eapply IHargs; eauto.
+    inv H0. assumption.
+Qed.
+
+Lemma value_inject_unchanged_on :
+  forall m m',
+    Mem.unchanged_on all_addrs m m' ->
+    forall {A B} (ge : Genv.t A B) v v',
+      value_inject ge m v v' ->
+      value_inject ge m' v v'.
+Proof.
+  induction v using value_ind';
+      intros;
+  inv H1; econstructor;
+    try (eapply loadv_unchanged_on; eauto);
+    try (eapply load_all_unchanged_on; eauto);
+    try (intros; eapply value_inject_load_all; eauto);
+    eauto.
+Qed.
+  
+
+Lemma unchanged_env_inject :
+  forall {A B} (ge : Genv.t A B) e e' m m',
+    env_inject e e' ge m ->
+    Mem.unchanged_on all_addrs m m' ->
+    env_inject e e' ge m'.
+Proof.
+  intros.
+  unfold env_inject in *.
+  intros. eapply H in H1.
+  break_exists; break_and. exists x; split; auto.
+  inv H2; econstructor; eauto;
+    try (eapply loadv_unchanged_on; eauto);
+    try (eapply load_all_unchanged_on; eauto);
+    try (intros; eapply value_inject_unchanged_on; eauto).
+Qed.
+
+
+Lemma store_value_res :
+  forall {A B} v m v' m' (ge : Genv.t A B),
+    store_value ge v m = Some (v',m') ->
+    exists b ofs,
+      v' = Vptr b ofs.
+Proof.
+  intros.
+  destruct v;
+    unfold store_value in *; fold (@store_value A B) in *;
+      fold (@store_values A B) in *;
+      repeat (break_match_hyp; try congruence);
+      inv H;
+      eexists; eexists; reflexivity.
+Qed.
+
+
+Lemma store_value_inject :
+  forall {A B} (ge : Genv.t A B) v v' m m' ,
+    store_value ge v m = Some (v',m') ->
+    value_inject ge m' v v'.
+Proof.
+  (* Holy Hell *)
+  intros A B ge.
+  induction v using value_rect_mut with
+  (Pl := fun l =>
+      forall b z m m',
+        store_values ge b z l m = Some m' ->
+        exists l',
+          load_all (arg_addrs b (Int.repr z) l) m' = Some l' /\
+        forall a b,
+          (In (a,b) l' -> value_inject ge m' a b));
+    intros.
+  * unfold store_value in H; fold (@store_value A B) in H.
+    fold (@store_values A B) in H.
+    break_let. repeat (break_match_hyp; try congruence).
+    invc H.
+    eapply IHv in Heqo0.
+    break_exists. break_and.
+    econstructor; eauto.
+    (* just store isolation *)
+    admit.
+
+  * unfold store_value in H. fold store_value in H.
+    fold store_values in H.
+    break_let. repeat (break_match_hyp; try congruence).
+    invc H.
+    eapply IHv in Heqo2.
+    break_exists. break_and.
+    econstructor; eauto.
+    (* just store isolation *)
+    admit.
+  * simpl in H. inv H.
+    simpl. exists [].
+    split; intros; eauto.
+    simpl in *. inv H0.
+  * simpl in H.
+    repeat (break_match_hyp; try congruence).
+    subst p.
+    remember Heqo as Hstorevals.
+    remember Heqo0 as Hstoreval.
+    clear HeqHstoreval.
+    clear HeqHstorevals.
+    eapply IHv in Heqo0.
+    eapply IHv0 in Heqo.
+    break_exists. break_and.
+    exists ((v,v0) :: x).
+    split; intros.
+    simpl.
+    assert (Mem.load Mint32 m' b (Int.unsigned (Int.repr z)) = Some v0).
+    {
+      eapply Mem.load_store_same in H. rewrite H.
+      f_equal.
+      eapply store_value_res in Hstoreval.
+      repeat break_exists. subst v0. simpl.
+      reflexivity.
+    } idtac.
+    rewrite H2.
+    replace (Int.repr (z + 4)) with (Int.add (Int.repr z) (Int.repr 4)) in H0.
+
+    (* m0 -store_value> m1 -Mem.store> m' *)
+    (* Lemma: load all passes over store_value *)
+    (* Lemma: load all passes over store *)
+    admit.
+
+    rewrite Int.add_unsigned.
+    eapply Int.eqm_samerepr.
+    eapply Int.eqm_add.
+    eapply Int.eqm_unsigned_repr_l. eapply Int.eqm_refl.
+    eapply Int.eqm_unsigned_repr_l. eapply Int.eqm_refl.
+
+    simpl in H2. destruct H2.
+    invc H2.
+
+    (* m1 -Mem.store> m' *)
+    (* Lemma value_inject passes over Mem.store *)
+    (* We need some extra info to prove this, not sure it's present here *)
+    admit. 
+
+
+    remember H2 as Hin.
+    clear HeqHin.
+    eapply H1 in H2.
+    (* m0 -store_value> m1 -Mem.store> m' *)
+    (* Lemma: value_inject passes over store_value *)
+    (* Lemma: value_inject passes over Mem.store *)
+    admit.
+    
+Admitted.
+
+(* This is the cool one *)
+(* if we Set in Emajor land, what operation is that in Dmajor? *)
+Lemma env_inject_set :
+  forall {A B} e e' (m : mem) (ge : Genv.t A B),
+    env_inject e e' ge m ->
+    forall v v' m',
+      store_value ge v m = Some (v',m') ->
+      forall id,
+        env_inject (PTree.set id v e) (PTree.set id v' e') ge m'.
+Proof.
+  intros.
+  unfold env_inject in *. intros.
+  destruct (peq id id0).
+
+  Focus 2. rewrite PTree.gso in * by congruence.
+  eapply H in H1. break_exists. break_and.
+  exists x. split; eauto. eapply value_inject_unchanged_on; eauto.
+  eapply store_value_unchanged; eauto.
+
+  subst id.
+  rewrite PTree.gss in *.
+  inv H1. exists v'.
+  split; auto.
+  eapply store_value_inject; eauto.
+Qed.
+
+
